test_coq/deque.v
@@ -1,4 +1,4 @@
-From Cadeque.deque Require Import core.
+From Cadeque.deque Require Import deque.
 
 Definition test : option (deque nat * nat) :=
   let d := proj1_sig empty in
@@ -12,5 +12,37 @@ Definition test : option (deque nat * nat) :=
   | Some (_, d) => proj1_sig (eject d)
   | None => None
   end.
+
+Eval vm_compute in test.
+
+From Cadeque.deque Require Import deque_lvl.
+
+Definition test_lvl : option (deque nat * nat) :=
+  let d := proj1_sig empty in
+  let d := proj1_sig (push 2 d) in
+  let d := proj1_sig (push 1 d) in
+  let d := proj1_sig (push 0 d) in
+  let d := proj1_sig (inject d 3) in
+  let d := proj1_sig (inject d 4) in
+  let d := proj1_sig (inject d 5) in
+  match proj1_sig (pop d) with
+  | Some (_, d) => proj1_sig (eject d)
+  | None => None
+  end.
+
+Eval vm_compute in test.
+
+From Cadeque.deque Require Import deque_size.
+
+Definition test_size : deque nat 4 * nat :=
+  let d := proj1_sig empty in
+  let d := proj1_sig (push 2 d) in
+  let d := proj1_sig (push 1 d) in
+  let d := proj1_sig (push 0 d) in
+  let d := proj1_sig (inject d 3) in
+  let d := proj1_sig (inject d 4) in
+  let d := proj1_sig (inject d 5) in
+  let '(_, d) := proj1_sig (pop d) in
+  proj1_sig (eject d).
 
 Eval vm_compute in test.
